Weidenbach_Book/IsaSAT/IsaSAT_Watch_List.thy
@@ -77,14 +77,14 @@ type_synonym nat_clauses_l = \<open>nat list list\<close>
 subsubsection \<open>Refinement of the Watched Function\<close>
 
 definition watched_by_nth :: \<open>nat twl_st_wl \<Rightarrow> nat literal \<Rightarrow> nat \<Rightarrow> nat watcher\<close> where
-  \<open>watched_by_nth = (\<lambda>(M, N, D, NE, UE, NS, US, Q, W) L i. W L ! i)\<close>
+  \<open>watched_by_nth = (\<lambda>(M, N, D, NE, UE, NS, US, N0, U0, Q, W) L i. W L ! i)\<close>
 
 definition watched_app
   :: \<open>(nat literal \<Rightarrow> (nat watcher) list) \<Rightarrow> nat literal \<Rightarrow> nat \<Rightarrow> nat watcher\<close> where
   \<open>watched_app M L i \<equiv> M L ! i\<close>
 
 lemma watched_by_nth_watched_app:
-  \<open>watched_by S K ! w = watched_app ((snd o snd o snd o snd o snd o snd o snd o snd) S) K w\<close>
+  \<open>watched_by S K ! w = watched_app ((snd o snd o snd o snd o snd o snd o snd o snd o snd o snd) S) K w\<close>
   by (cases S) (auto simp: watched_app_def)
 
 
